CoqOfRust/_std/slice.v
@@ -1,23 +1,6 @@
 Require Import CoqOfRust.lib.lib.
 
 Require Import CoqOfRust._std.option.
-Require Import CoqOfRust._std.vec.
-
-Module hack.
-  Parameter t : Set.
-
-  Parameter into_vec : forall {T A : Set} `{core.alloc.Allocator.Trait A}
-    {(* TODO: use (Box (Slice T) A) instead of X *) X : Set} (b : X),
-      Vec T (Some A).
-End hack.
-Definition hack := hack.t.
-
-Module hack_notations.
-  Global Instance hack_into_vec {T A : Set} `{core.alloc.Allocator.Trait A}
-    {X : Set} : Notation.DoubleColon hack "into_vec" := {
-    Notation.double_colon (b : X) := hack.into_vec (T := T) (A := A) b;
-  }.
-End hack_notations.
 
 (* ********STRUCTS******** *)
 (*
@@ -444,20 +427,3 @@ End SliceIndex.
 [ ] from_raw_parts_mut
 [ ] from_ref
 *)
-
-(* *****IMPLEMENTATIONS***** *)
-Module Impl_Slice.
-  Section Impl_Slice.
-    Parameter T : Set.
-    Definition Self := slice T.
-
-    Definition into_vec {A : Set} `{core.alloc.Allocator.Trait A}
-      (self : ref Self) (alloc : A) : Vec T (Some A) :=
-        hack::["into_vec"] self.
-
-    Global Instance Method_into_vec {A : Set} `{core.alloc.Allocator.Trait A} :
-      Notation.DoubleColon slice "into_vec" := {
-        Notation.double_colon (self : ref Self) (alloc : A) := into_vec self alloc;
-      }.
-  End Impl_Slice.
-End Impl_Slice.
